AddOns/AngelicVerifierNull/test/propinst-regressions/null0.bpl
@@ -1,0 +1,12 @@
+const NULL: int;
+
+procedure foo({:pointer} x: int)
+{
+  var ax: int;
+
+  ax := x;
+  if(*) { ax := NULL; }
+  assume {:nonnull} ax != NULL; 
+}
+
+
